Add Exthtbl and implement typevar to string correctly
Tiny bit of state monad start

extract/Exthtbl2.mli
@@ -1,0 +1,27 @@
+open CoqHashtbl
+open Datatypes
+open StateMonad
+open Extmap
+
+module type S =
+ sig
+  type key
+
+  type value
+
+  type t
+
+  val create : Int.t -> unit
+
+  val add : key -> value -> unit
+
+  val find_opt : key -> value option
+ end
+
+module type TyMod =
+ sig
+  type t
+ end
+
+module Make (X:TaggedType) (Y:TyMod) :
+    S with type key = X.t with type value = Y.t
