src/coqutil/Ctr.v
@@ -1,0 +1,18 @@
+(*A counter, mutable when extracted to OCaml.
+  We put it in a module so that multiple instances can be created*)
+Require Import StateMonad.
+From ExtLib Require Import StateMonad.
+(* Notation ctr := (state CoqBigInt.t). *)
+Module Type Ctr.
+Parameter create : CoqBigInt.t -> state CoqBigInt.t unit.
+Parameter incr : unit -> ctr unit.
+Parameter get : unit -> ctr CoqBigInt.t. (*Important - in state monad*)
+End Ctr.
+
+Module MakeCtr <: Ctr.
+Definition ctr_ref : ctr_ty := new_ctr CoqBigInt.zero.
+Definition create (i: CoqBigInt.t) : ctr unit :=
+  ctr_set i.
+Definition incr (_: unit) : ctr unit := ctr_incr.
+Definition get (_: unit) : ctr CoqBigInt.t := ctr_get.
+End MakeCtr.
