src/util/CoqExthtbl.v
@@ -1,0 +1,50 @@
+Require Import CoqInt.
+Require Import StateMonad.
+Require Import CoqHashtbl.
+(*TODO: is this bad?*)
+Require Import CoqWstdlib.
+Module Type S.
+
+(*Very limited for now - create, add, find*)
+(*We have a different interface in 2 ways:
+  1. We do not expose the table, so only 1 hash table
+    can be created per type.
+  2. These are NOT polymorphic: they are specialized
+    to a particular module type. Otherwise, we run into
+    problems with OCaml weak variables and the value
+    restriction.*)
+Parameter key : Type.
+Parameter value : Type.
+Parameter t : Type.
+
+Section Ty.
+
+(* Parameter create : CoqInt.int -> hash_st key a (t a). *)
+Parameter create : CoqInt.int -> hash_st key value unit.
+Parameter add : key -> value -> hash_st key value unit.
+Parameter find_opt : key -> hash_st key value (option value).
+End Ty.
+End S.
+
+Module Type TyMod.
+Parameter t : Type.
+End TyMod.
+
+Module Make (X: TaggedType) (Y: TyMod) <: S.
+Definition key := X.t.
+Definition value := Y.t.
+
+Definition t : Type := hashtbl key value.
+
+Definition hash_ref : hash_unit := @new_hash key value.
+
+Section Ty.
+Definition create (_: CoqInt.int) : hash_st key value unit :=
+  hash_set (create_hashtbl value).
+Definition add (k: key) (v: value) : hash_st key value unit :=
+  hash_bnd (fun h => hash_set (add_hashtbl X.tag h k v)) hash_get.
+Definition find_opt (k: key) : hash_st key value (option value) :=
+  hash_bnd (fun h => hash_ret 
+    (option_map snd (find_opt_hashtbl X.tag X.equal h k))) hash_get.
+End Ty.
+End Make.
